theories/Lowering/LabelRelations.v
@@ -1,0 +1,70 @@
+Require Import Util Get Linear.
+
+Definition not_contains_label C l :=
+  forall n l', get C n (Llabel l') -> l' <> l.
+
+Definition all_labels_smaller C l :=
+  forall n l', get C n (Llabel l') -> (l' < l)%positive.
+
+Definition all_labels_ge C l :=
+  forall n l', get C n (Llabel l') -> (l <= l')%positive.
+
+Lemma all_not_labels C l
+  : all_labels_smaller C l
+    ->  not_contains_label C l.
+Proof.
+  intros. hnf; intros. exploit H; eauto.
+  intro. subst.
+  eapply Pos.lt_irrefl. eauto.
+Qed.
+
+Lemma all_not_labels_ge C l
+  : all_labels_ge C (Pos.succ l)
+    -> not_contains_label C l.
+Proof.
+  intros. hnf; intros. exploit H; eauto.
+  intro. subst.
+  eapply Pos.le_succ_l in H1.
+  eapply Pos.lt_irrefl. eauto.
+Qed.
+
+Hint Resolve all_not_labels.
+
+Lemma not_contains_label_app1 C C' l
+  : not_contains_label C l -> not_contains_label C' l -> not_contains_label (C ++ C') l.
+Proof.
+  intros; hnf; intros.
+  eapply get_app_cases in H1 as [? |[? ?]]; eauto.
+Qed.
+
+Lemma all_labels_smaller_app1 C C' l
+  : all_labels_smaller C l -> all_labels_smaller C' l -> all_labels_smaller (C ++ C') l.
+Proof.
+  intros; hnf; intros.
+  eapply get_app_cases in H1 as [? |[? ?]]; eauto.
+Qed.
+
+Lemma all_labels_ge_app1 C C' l
+  : all_labels_ge C l -> all_labels_ge C' l -> all_labels_ge (C ++ C') l.
+Proof.
+  intros; hnf; intros.
+  eapply get_app_cases in H1 as [? |[? ?]]; eauto.
+Qed.
+
+Lemma all_labels_smaller_le C l l'
+  : all_labels_smaller C l
+    -> (l <= l')%positive
+    -> all_labels_smaller C l'.
+Proof.
+  intros; hnf; intros.
+  eapply H in H1. eapply Pos.lt_le_trans; eauto.
+Qed.
+
+Lemma all_labels_ge_le C l l'
+  : all_labels_ge C l
+    -> (l' <= l)%positive
+    -> all_labels_ge C l'.
+Proof.
+  intros; hnf; intros.
+  eapply H in H1. etransitivity; eauto.
+Qed.
