theories/Lowering/LinearStateType.v
@@ -1,0 +1,120 @@
+Require Import Coqlib Errors AST Integers Linear.
+Require Import Bounds Conventions Locations Stacklayout.
+Require Import Smallstep Globalenvs common.Events.
+Require Import Util Get StateType SmallStepRelations IL.Events.
+
+Set Implicit Arguments.
+
+Inductive linear_step_adapter (G:Globalenvs.Genv.t fundef unit)
+  :  Linear.state -> Events.event -> Linear.state -> Prop :=
+| StepAdapterTau st bv vv code rs m σ'
+  : Linear.step G (State st bv vv code rs m) nil σ'
+    -> linear_step_adapter G (State st bv vv code rs m)  EvtTau σ'
+| StepAdapter σ σ' f arg res fnc
+  : Linear.step G σ (Event_syscall f
+                               (EVint ⊝ arg)
+                               (EVint res)::nil) σ'
+    -> linear_step_adapter G σ (EvtExtern (ExternI fnc arg res)) σ'.
+
+Lemma linear_reddec2 G
+  : reddec2 (linear_step_adapter G).
+Proof.
+  hnf; intros.
+  unfold normal2.
+  eapply Coq.Logic.Classical_Prop.classic.
+Defined.
+
+Definition linear_result (σ:Linear.state) :=
+  match σ with
+  | Returnstate st rs m =>
+    match Locmap.get (R R3) rs with
+    | Values.Vint retcode => Some retcode
+    | _ => None
+    end
+  | _ => None
+  end.
+
+Lemma list_forall_det A B (R:A->B->Prop) L L1 L2
+      (Rdet: forall x y z, R x y -> R x z -> y = z)
+  : list_forall2 R L L1
+    -> list_forall2 R L L2
+    -> L1 = L2.
+Proof.
+  intros X Y.
+  general induction X; invt list_forall2; eauto.
+  f_equal; eauto.
+Qed.
+
+(*
+Lemma extcall_arg_det rs m sp l v v'
+  : extcall_arg rs m sp l v
+    -> extcall_arg rs m sp l v'
+    -> v = v'.
+Proof.
+  intros A B.
+  general induction A; invt extcall_arg; eauto.
+  congruence.
+Qed.
+ *)
+(*
+Lemma extcall_arguments_det rs m sp ef a a'
+  : extcall_arguments rs m sp ef a
+    -> extcall_arguments rs m sp ef a'
+    -> a = a'.
+Proof.
+  eapply list_forall_det.
+  intros. general induction H; invt extcall_arg_pair; f_equal; eauto using extcall_arg_det.
+Qed.
+ *)
+
+Local Ltac congr :=
+  repeat match goal with
+         | [ H : ?t = ?x, H' : ?t = ?y |- _ ] =>
+           assert (x = y) by congruence; subst; clear H' || clear H
+         | [ H : eval_builtin_args ?G ?rs ?sp ?m ?a ?vargs,
+                 H' :  eval_builtin_args ?G ?rs ?sp ?m ?a ?vargs' |- _ ]
+           => eapply eval_builtin_args_determ in H; eauto; subst
+(*         | [ H : extcall_arguments ?rs ?m ?sp ?ef ?a,
+               H' : extcall_arguments ?rs ?m ?sp ?ef ?a' |- _ ]
+         => eapply extcall_arguments_det in H; eauto; subst*)
+
+         | [ H :  external_call ?ef ?G ?vargs ?m ?t ?vres ?m',
+                  H' :   external_call ?ef ?G ?vargs ?m ?t' ?vres' ?m'' |- _ ]
+
+           =>  let A := fresh "A" in
+              let B := fresh "B" in
+              edestruct (external_call_determ _ _ _ _ _ _ _ _ _ _ H H') as [A B];
+              inv A; try (edestruct B; eauto; subst); clear H || clear H'
+         | [ s := _ |- _ ] => subst s
+         end.
+
+Definition rel3_functional {A B C} (R:A->B->C->Prop) :=
+  forall a b c c', R a b c -> R a b c' -> c = c'.
+
+Lemma linear_int_det G
+  : internally_deterministic (linear_step_adapter G).
+Proof.
+  hnf; intros.
+  inv H; inv H0; eauto.
+  - inv H1; inv H10; congr; clear_trivial_eqs; try now (split; eauto; congr; try congruence).
+
+  - inv H1; inv H2; exfalso; repeat (congr; clear_trivial_eqs).
+Qed.
+
+Lemma linear_ext_det G
+  : externally_determined (linear_step_adapter G).
+Proof.
+  hnf. intros.
+  invc H; invc H0; eauto.
+  - inv H1; inv H8; repeat (congr; clear_trivial_eqs);
+      try now (split; eauto; congr; try congruence).
+  - inv H1; inv H6; repeat (congr; clear_trivial_eqs); eauto.
+Qed.
+
+Instance LinearStateType G : StateType Linear.state :=
+  @Build_StateType _ (linear_step_adapter G) linear_result (linear_reddec2 G)
+                   (@linear_int_det G) (@linear_ext_det G).
+
+Ltac single_step_linear := econstructor; econstructor; eauto.
+
+Smpl Add single_step_linear : single_step.
