theories/Lowering/MkVars.v
@@ -1,0 +1,61 @@
+Require Import Util Var Get Coqlib.
+
+Set Implicit Arguments.
+
+Fixpoint mkVars X (L:list X) (f:var) : var * list var :=
+  match L with
+  | nil => (f, nil)
+  | _::L => let f' := Pos.succ f in
+           let (f'', xl) := mkVars L f' in
+           (f'', f::xl)
+  end.
+
+
+Lemma mkVars_length X (L:list X) f
+  : ❬snd (mkVars L f)❭ = ❬L❭.
+Proof.
+  general induction L; simpl; repeat let_pair_case_eq; eauto; subst; simpl.
+  rewrite IHL; eauto.
+Qed.
+
+Smpl Add match goal with
+         | [ H : context [ ❬snd (@mkVars ?X ?L ?f)❭ ] |- _ ]
+           => setoid_rewrite (@mkVars_length X L f) in H
+         | [ |- context [ ❬snd (@mkVars ?X ?L ?f)❭ ] ]
+           => setoid_rewrite (@mkVars_length X L f)
+         end : len.
+
+Lemma mkVars_le X L f
+  : (f <= fst (@mkVars X L f))%positive.
+Proof.
+  general induction L; simpl.
+  - reflexivity.
+  - let_pair_case_eq; simpl_pair_eqs; subst; simpl.
+    rewrite <- IHL. eapply Ple_succ.
+Qed.
+
+Lemma mkVars_get_le X (L:list X) f n i
+  :  get (snd (mkVars L f)) n i
+     -> (f <= i)%positive.
+Proof.
+  intros GET.
+  general induction L; simpl in *.
+  - isabsurd.
+  - revert GET; let_pair_case_eq; simpl_pair_eqs; subst; simpl.
+    intros GET. inv GET.
+    + reflexivity.
+    + eapply IHL in H3. rewrite <- H3. eapply Ple_succ.
+Qed.
+
+Lemma mkVars_get_lt X (L:list X) f n i
+  :  get (snd (mkVars L f)) n i
+     -> (i < fst (mkVars L f))%positive.
+Proof.
+  intros GET.
+  general induction L; simpl in *.
+  - isabsurd.
+  - revert GET; let_pair_case_eq; simpl_pair_eqs; subst; simpl.
+    intros GET. inv GET.
+    + eapply Pos.lt_le_trans. eapply Plt_succ. rewrite <- mkVars_le. reflexivity.
+    + eapply IHL; eauto.
+Qed.
